I got it verified with ADT

SlowTest/SmallestMissingNumber-functional-adt.dfy
@@ -17,9 +17,9 @@ datatype List<X> = Nil | Cons(head: X, tail: List<X>)
 // const {:extern} Ab8 : AbInt
 
 function method int2adt (n: int) : (r: AbInt)
-predicate IsZero (n: AbInt) {n == int2adt(0)}
-predicate NonNeg (n: AbInt) { true }
-predicate AbPos (n: AbInt) {NonNeg(n) && !IsZero(n)}
+predicate AbIsZero (n: AbInt) {n == int2adt(0)}
+predicate AbNonNeg (n: AbInt) { true }
+predicate AbPos (n: AbInt) {AbNonNeg(n) && !AbIsZero(n)}
 
 function method AbLt(n: AbInt, m: AbInt) : bool
 function method AbAdd(n: AbInt, m: AbInt) : (r: AbInt)
@@ -28,42 +28,69 @@ function method AbAdd(n: AbInt, m: AbInt) : (r: AbInt)
 // TODO: if len is also an ADT, what should I do here?
 function method AbBoundSet(lo: AbInt, len: nat): (S: set<AbInt>)
   ensures |S| == len
-  ensures S == set x | 0 <= x < len :: AbAdd(lo, int2adt(x))
+  ensures forall x :: (AbLt(lo, x) || lo == x) && AbLt(x, AbAdd(lo, int2adt(len)))
+  // Try not to assign every element with AbAdd()
+  // ensures S == set x | 0 <= x < len :: AbAdd(lo, int2adt(x))
 
 
 /* Properties */
-lemma Props()
-  /* AbLt */
-  ensures forall x, y, z :: AbLt(x, y) && AbLt(y, z) ==> AbLt(x, z)
-  // ensures forall n :: !AbLt(n, n)
-  // ensures forall x, y :: AbPos(y) ==> AbLt(x, AbAdd(x, y))
-  ensures forall x, y :: AbLt(x, y) <==> !(AbLt(y, x) || x == y)
+lemma Prop_all_leq_zero ()
   ensures forall x :: AbLt(int2adt(0), x) || x == int2adt(0)
-  // ensures forall x : AbInt, y : int :: y != 0 ==> AbLt (x, AbAdd(x, int2adt(y)))
-  ensures forall x, y, z :: AbLt(y, z) ==> AbLt(AbAdd(x, y), AbAdd(x, z))
-  // TODO: may not have integer here?
-  ensures forall x, y : int :: x < y ==> AbLt(int2adt(x), int2adt(y))
+lemma Props_lt_is_not_geq ()
+  ensures forall x, y :: AbLt(x, y) <==> !(AbLt(y, x) || x == y)
+lemma Props_lt_addition () // trigger problem?
+  ensures forall x, a, b:: AbLt(a, b) ==> AbLt(AbAdd(x, a), AbAdd(x, b))
+lemma Props_lt_transitive ()
+  ensures forall x, y, z :: AbLt(x, y) && AbLt(y, z) ==> AbLt(x, z)
+lemma Props_plus_zero ()
+  ensures forall x :: AbAdd(x, int2adt(0)) == AbAdd(int2adt(0), x) == x
+lemma Props_eq_less_is_lt ()
+  ensures forall x, y, a, b :: (x == AbAdd(y, a)) && AbLt(a, b) ==> AbLt(x, AbAdd(y, b))
+lemma Props_plus_eq_is_lt ()
+  ensures forall x, y, a :: (AbAdd(x, a) == y) && AbNonNeg(a) ==> AbLt(x, y)
+lemma Props_plus_lt_is_lt ()
+  ensures forall x, y, a :: AbLt(AbAdd(x, a), y) && AbNonNeg(a) ==> AbLt(x, y)
+lemma Props_plus_pos_is_neq ()
+  ensures forall x, a :: AbPos(a) ==> AbAdd(x, a) != x
+lemma Props_one_in_bound ()
+  ensures forall a, x :: (AbLt(a, x) || a == x) && (AbLt(x, AbAdd(a, int2adt(1)))) ==> a == x
+lemma Props_plus_minus_is_eq ()
+  ensures forall x: AbInt, i, j: int :: AbAdd(AbAdd(x, int2adt(j)), int2adt(i-j)) == AbAdd(x, int2adt(i)) // trigger may loop
 
-  /* AbAdd */
-  // ensures forall x, y :: AbAdd(x, y) == AbAdd(y, x)
-  // ensures forall x, y, z :: AbAdd(AbAdd(x, y), z) == AbAdd(x, AbAdd(y, z))
-  // ensures forall x :: AbAdd(x, int2adt(0)) == AbAdd(int2adt(0), x) == x
-  ensures forall x : AbInt, y, z : int :: AbAdd(AbAdd(x, int2adt(y)), int2adt(z-y)) == AbAdd(x, int2adt(z)) // trigger may loop
+lemma Props_int_pos(a: int)
+  ensures AbPos(int2adt(a))
+lemma Props_int_cmp_lt(a: int, b: int) // Lt(s, n+?) ==> Lt(s, n+?)
+  ensures AbLt(int2adt(a), int2adt(b))
+// Props_eq_less_is_lt_param(s, n, int2adt(llen), int2adt(len));
+lemma Props_eq_less_is_lt_param (x: AbInt, y: AbInt, a: AbInt, b: AbInt)
+  ensures (x == AbAdd(y, a)) && AbLt(a, b) ==> AbLt(x, AbAdd(y, b))
+// Props_plus_minus_is_eq_param(n, llen, len);
+lemma Props_plus_minus_is_eq_param(x: AbInt, i: int, j: int)
+  ensures AbAdd(AbAdd(x, int2adt(j)), int2adt(i-j)) == AbAdd(x, int2adt(i)) // trigger may loop
 
-lemma Props2()
-  ensures forall x, y, n1, n2 :: (AbAdd(y, n1) == x) && AbLt(n1, n2) ==> AbLt(x, AbAdd(y, n2))
-  ensures forall x, y, n :: AbAdd(y, n) == x ==> AbLt(y, x) || y == x
-
-lemma Set_Props(S1 : set<AbInt>, n: AbInt, l: nat)
-  /* Set */
-  ensures var S2 := AbBoundSet(n, l);
-    forall x :: x in S1 && AbLt(x, AbAdd(n, int2adt(l))) ==> S1 <= S2
-
-lemma Set_Props2 (xs: set<AbInt>, b: AbInt, s: AbInt)
-  ensures
-    var S1 := (set x | x in xs && AbLt(x, b));
-    var S2 := (set x | x in xs && !AbLt(x, b));
-    s !in S1 ==> s !in xs
+lemma Props ()
+  // Prop_all_leq_zero ()
+  ensures forall x :: AbLt(int2adt(0), x) || x == int2adt(0)
+  // Props_lt_is_not_geq ()
+  ensures forall x, y :: AbLt(x, y) <==> !(AbLt(y, x) || x == y)
+  // Props_lt_addition ()
+  ensures forall x, a, b:: AbLt(a, b) ==> AbLt(AbAdd(x, a), AbAdd(x, b))
+  // Props_lt_transitive ()
+  ensures forall x, y, z :: AbLt(x, y) && AbLt(y, z) ==> AbLt(x, z)
+  // Props_plus_zero ()
+  ensures forall x :: AbAdd(x, int2adt(0)) == AbAdd(int2adt(0), x) == x
+  // Props_eq_less_is_lt ()
+  ensures forall x, y, a, b :: (x == AbAdd(y, a)) && AbLt(a, b) ==> AbLt(x, AbAdd(y, b))
+  // Props_plus_eq_is_lt ()
+  ensures forall x, y, a :: (AbAdd(x, a) == y) && AbNonNeg(a) ==> AbLt(x, y)
+  // Props_plus_lt_is_lt ()
+  ensures forall x, y, a :: AbLt(AbAdd(x, a), y) && AbNonNeg(a) ==> AbLt(x, y)
+  // Props_plus_pos_is_neq ()
+  ensures forall x, a :: AbPos(a) ==> AbAdd(x, a) != x
+  // Props_one_in_bound ()
+  ensures forall a, x :: (AbLt(a, x) || a == x) && (AbLt(x, AbAdd(a, int2adt(1)))) ==> a == x
+  // Props_plus_minus_is_eq ()
+  ensures forall x: AbInt, i, j: int :: AbAdd(AbAdd(x, int2adt(j)), int2adt(i-j)) == AbAdd(x, int2adt(i)) 
 
 method Main() {
   var xs := Nil;
@@ -98,50 +125,49 @@ function method SMN(xs: List<AbInt>, n: AbInt, len: nat): AbInt
   decreases len
 {
   if 2 <= len then
-    var (L, R) := Split(xs, AbAdd(n, int2adt(len/2))); // ADT
+    var (L, R) := Split(xs, AbAdd(n, int2adt(len/2)));
     var llen := Length(L);
     if llen < len/2 then
       SMN(L, n, llen)
     else
-      SMN(R, AbAdd(n, int2adt(llen)), len - llen) // ADT
+      SMN(R, AbAdd(n, int2adt(llen)), len - llen)
   else if xs.Cons? then
-    if xs.head == n then AbAdd(n, int2adt(1)) else n // ADT
+    if xs.head == n then AbAdd(n, int2adt(1)) else n
   else
     n
 }
 
-// verified
-// function method SMN'(xs: List<AbInt>, n: AbInt, len: nat): AbInt
-//   requires len == Length(xs)
-//   decreases len
-// {
-//   if xs == Nil then
-//     n
-//   else
-//     var half := (len + 1) / 2;
-//     var (L, R) := Split(xs, AbAdd(n, int2adt(half)));
-//     var llen := Length(L);
-//     if llen < half then
-//       SMN'(L, n, llen)
-//     else
-//       SMN'(R, AbAdd(n, int2adt(llen)), len - llen)
-// }
+function method SMN'(xs: List<AbInt>, n: AbInt, len: nat): AbInt
+  requires len == Length(xs)
+  decreases len
+{
+  if xs == Nil then
+    n
+  else
+    var half := (len + 1) / 2;
+    var (L, R) := Split(xs, AbAdd(n, int2adt(half)));
+    var llen := Length(L);
+    if llen < half then
+      SMN'(L, n, llen)
+    else
+      SMN'(R, AbAdd(n, int2adt(llen)), len - llen)
+}
 
-// function method SMN''(xs: List<AbInt>, n: AbInt, len: nat): AbInt
-//   requires len == Length(xs)
-//   decreases len
-// {
-//   if xs == Nil then
-//     n
-//   else
-//     var half := len / 2 + 1;
-//     var (L, R) := Split(xs, AbAdd(n, int2adt(half)));
-//     var llen := Length(L);
-//     if llen < half then
-//       SMN''(L, n, llen)
-//     else
-//       SMN''(R, AbAdd(n, int2adt(llen)), len - llen)
-// }
+function method SMN''(xs: List<AbInt>, n: AbInt, len: nat): AbInt
+  requires len == Length(xs)
+  decreases len
+{
+  if xs == Nil then
+    n
+  else
+    var half := len / 2 + 1;
+    var (L, R) := Split(xs, AbAdd(n, int2adt(half)));
+    var llen := Length(L);
+    if llen < half then
+      SMN''(L, n, llen)
+    else
+      SMN''(R, AbAdd(n, int2adt(llen)), len - llen)
+}
 
 function method Split(xs: List<AbInt>, b: AbInt): (List<AbInt>, List<AbInt>)
   ensures var r := Split(xs, b); Length(xs) == Length(r.0) + Length(r.1)
@@ -150,7 +176,7 @@ function method Split(xs: List<AbInt>, b: AbInt): (List<AbInt>, List<AbInt>)
   case Nil => (Nil, Nil)
   case Cons(x, tail) =>
     var (L, R) := Split(tail, b);
-    if AbLt(x, b) then // ADT
+    if AbLt(x, b) then
       (Cons(x, L), R)
     else
       (L, Cons(x, R))
@@ -216,11 +242,11 @@ lemma SetEquality(A: set, B: set)
 function IntRange(lo: AbInt, len: nat): set<AbInt>
   ensures |IntRange(lo, len)| == len
 {
-  var S := AbBoundSet(lo, len); // ADT
-  assert len != 0 ==> S == IntRange(lo, len - 1) + {AbAdd(lo, int2adt(len - 1))}; // ADT
-  // TODO: can we check this with Props()? Nop, because we don't know AbLt(int2adt(x), int2adt(y))
-  // Props ();
-  // assert forall x :: x in S ==> (AbLt(lo, x) || lo == x) && AbLt(x, AbAdd(lo, int2adt(len)));
+  var S := AbBoundSet(lo, len);
+  assume AbLt(int2adt(len - 1), int2adt(len));
+  // Try not to assign every element with AbAdd()
+  // assert len != 0 ==> S == IntRange(lo, len - 1) + {AbAdd(lo, int2adt(len - 1))};
+  assert forall x :: x in S ==> (AbLt(lo, x) || lo == x) && AbLt(x, AbAdd(lo, int2adt(len)));
   S
 }
 
@@ -232,7 +258,7 @@ lemma SmallestMissingNumber_Correct(xs: List<AbInt>)
     s !in Elements(xs) &&
     forall x :: (AbLt(int2adt(0), x) || int2adt(0) == x) && AbLt(x, s) ==> x in Elements(xs)
 {
-  Props ();
+  Prop_all_leq_zero ();
   SMN_Correct(xs, int2adt(0), Length(xs));
 }
 
@@ -242,33 +268,81 @@ lemma SMN_Correct(xs: List<AbInt>, n: AbInt, len: nat)
   requires forall x :: x in Elements(xs) ==> (AbLt(n, x) || n == x)
   requires len == Length(xs)
   ensures var s := SMN(xs, n, len);
-    (AbLt(n, s) || n == s) && // failed
-    (AbLt(s, AbAdd(n, int2adt(len))) || s == AbAdd(n, int2adt(len))) && // failed
-    s !in Elements(xs) && // failed
-    forall x ::(AbLt(n, x) || n == x) && AbLt(x, s) ==> x in Elements(xs) //failed
+    (AbLt(n, s) || n == s) &&
+    (AbLt(s, AbAdd(n, int2adt(len))) || s == AbAdd(n, int2adt(len))) &&
+    s !in Elements(xs) &&
+    forall x ::(AbLt(n, x) || n == x) && AbLt(x, s) ==> x in Elements(xs)
   decreases len
 {
+  Props ();
   if 2 <= len {
-    Props ();
     var (L, R) := Split(xs, AbAdd(n, int2adt(len/2)));
     Split_Correct(xs, AbAdd(n, int2adt(len/2)));
     var llen := Length(L);
-    Elements_Property(L);  // this is where we need the NoDuplicates property
+    Elements_Property(L);  // NoDuplicates property
     var bound := IntRange(n, len/2);
-    Set_Props(Elements(L), n, len/2); // ADT Props
+    // Props_lt_is_not_geq ();
     Cardinality(Elements(L), bound);
-    Props (); // Why I duplicate the assumptions here, it failed so quick?
     if llen < len/2 {
-      var s := SMN(L, n, llen);
+      // var s := SMN(L, n, llen);
       SMN_Correct(L, n, llen);
-      Set_Props2(Elements(xs), AbAdd(n, int2adt(len/2)), s);
-      Props2();
+      // Props_int_cmp_lt(llen, len); // Lt(s, n+llen) ==> Lt(s, n+len)
+      // Props_lt_addition ();
+      // Props_lt_transitive ();
+      // Props_eq_less_is_lt (); // s==n+llen ==> Lt(s, n+len)
     } else {
-      Props2();
       var s := SMN(R, AbAdd(n, int2adt(llen)), len - llen);
       SMN_Correct(R, AbAdd(n, int2adt(llen)), len - llen);
+      // Props_plus_lt_is_lt (); // Lt(n+llen, s) ==> Lt(n, s)      
+      // Props_plus_eq_is_lt (); // n+llen == s ==> Lt(n, s)
+      // Props_plus_minus_is_eq (); // (n+llen) + (len-llen) == n+len
       forall x | (AbLt(n, x) || n == x) && AbLt(x, s)
-        ensures x in Elements(xs) // failed
+        ensures x in Elements(xs)
+      {
+        if AbLt(x, AbAdd(n, int2adt(llen))) {
+          SetEquality(Elements(L), bound);
+        }
+      }
+    }
+  }
+  // else {
+  //   Props_plus_eq_is_lt ();
+  //   Props_int_pos(1);
+  //   Props_plus_pos_is_neq ();
+  //   Props_one_in_bound ();
+  //   Props_lt_is_not_geq ();
+  //   Props_plus_zero ();
+  // }
+}
+
+lemma SMN'_Correct(xs: List<AbInt>, n: AbInt, len: nat)
+  requires NoDuplicates(xs)
+  requires forall x :: x in Elements(xs) ==> (AbLt(n, x) || n == x)
+  requires len == Length(xs)
+  ensures var s := SMN'(xs, n, len);
+    (AbLt(n, s) || n == s) &&
+    (AbLt(s, AbAdd(n, int2adt(len))) || s == AbAdd(n, int2adt(len))) &&
+    s !in Elements(xs) &&
+    forall x :: (AbLt(n, x) || n == x) && AbLt(x, s) ==> x in Elements(xs)
+  decreases len
+{ 
+  Props ();
+  if xs == Nil {
+  } else {
+    var half := (len + 1) / 2;
+    var (L, R) := Split(xs, AbAdd(n, int2adt(half)));
+    Split_Correct(xs, AbAdd(n, int2adt(half)));
+    var llen := Length(L);
+    Elements_Property(L);  // use the NoDuplicates property
+    var bound := IntRange(n, half);
+    Cardinality(Elements(L), bound);
+    if llen < half {
+      SMN'_Correct(L, n, llen);
+    } else {
+      var s := SMN'(R, AbAdd(n, int2adt(llen)), len - llen);
+      SMN'_Correct(R, AbAdd(n, int2adt(llen)), len - llen);
+      forall x | (AbLt(n, x) || n == x) && AbLt(x, s)
+        ensures x in Elements(xs)
       {
         if AbLt(x, AbAdd(n, int2adt(llen))) {
           SetEquality(Elements(L), bound);
@@ -278,112 +352,39 @@ lemma SMN_Correct(xs: List<AbInt>, n: AbInt, len: nat)
   }
 }
 
-// // Here is an alternative version, with a different splitting
-// // condition (using the ceiling of len/2.0 instead of the floor)
-// // and only two cases.
-// function method SMN'(xs: List<nat>, n: nat, len: nat): nat
-//   requires len == Length(xs)
-//   decreases len
-// {
-//   if xs == Nil then
-//     n
-//   else
-//     var half := (len + 1) / 2;
-//     var (L, R) := Split(xs, n + half);
-//     var llen := Length(L);
-//     if llen < half then
-//       SMN'(L, n, llen)
-//     else
-//       SMN'(R, n + llen, len - llen)
-// }
-
-// // Here is yet one more version. This time, the splitting condition
-// // is 1 more than then floor of len/2.0. This is the version of the
-// // algorithm in Richard Bird's book.
-// function method SMN''(xs: List<nat>, n: nat, len: nat): nat
-//   requires len == Length(xs)
-//   decreases len
-// {
-//   if xs == Nil then
-//     n
-//   else
-//     var half := len / 2 + 1;
-//     var (L, R) := Split(xs, n + half);
-//     var llen := Length(L);
-//     if llen < half then
-//       SMN''(L, n, llen)
-//     else
-//       SMN''(R, n + llen, len - llen)
-// }
-
-// // ----- Proofs of alternative versions
-
-// lemma SMN'_Correct(xs: List<nat>, n: nat, len: nat)
-//   requires NoDuplicates(xs)
-//   requires forall x :: x in Elements(xs) ==> n <= x
-//   requires len == Length(xs)
-//   ensures var s := SMN'(xs, n, len);
-//     n <= s <= n + len &&
-//     s !in Elements(xs) &&
-//     forall x :: n <= x < s ==> x in Elements(xs)
-//   decreases len
-// {
-//   if xs == Nil {
-//   } else {
-//     var half := (len + 1) / 2;
-//     var (L, R) := Split(xs, n + half);
-//     Split_Correct(xs, n + half);
-//     var llen := Length(L);
-//     Elements_Property(L);  // use the NoDuplicates property
-//     var bound := IntRange(n, half);
-//     Cardinality(Elements(L), bound);
-//     if llen < half {
-//       SMN'_Correct(L, n, llen);
-//     } else {
-//       var s := SMN'(R, n + llen, len - llen);
-//       SMN'_Correct(R, n + llen, len - llen);
-//       forall x | n <= x < s
-//         ensures x in Elements(xs)
-//       {
-//         if x < n + llen {
-//           SetEquality(Elements(L), bound);
-//         }
-//       }
-//     }
-//   }
-// }
-
-// lemma SMN''_Correct(xs: List<nat>, n: nat, len: nat)
-//   requires NoDuplicates(xs)
-//   requires forall x :: x in Elements(xs) ==> n <= x
-//   requires len == Length(xs)
-//   ensures var s := SMN''(xs, n, len);
-//     n <= s <= n + len &&
-//     s !in Elements(xs) &&
-//     forall x :: n <= x < s ==> x in Elements(xs)
-//   decreases len
-// {
-//   if xs == Nil {
-//   } else {
-//     var half := len / 2 + 1;
-//     var (L, R) := Split(xs, n + half);
-//     Split_Correct(xs, n + half);
-//     var llen := Length(L);
-//     Elements_Property(L);  // use the NoDuplicates property
-//     var bound := IntRange(n, half);
-//     Cardinality(Elements(L), bound);
-//     if llen < half {
-//       SMN''_Correct(L, n, llen);
-//     } else {
-//       var s := SMN''(R, n + llen, len - llen);
-//       SMN''_Correct(R, n + llen, len - llen);
-//       forall x | n <= x < s
-//         ensures x in Elements(xs)
-//       {
-//         if x < n + llen {
-//           SetEquality(Elements(L), bound);
-//         }
-//       }
-//     }
-//   }
-// }
+lemma SMN''_Correct(xs: List<AbInt>, n: AbInt, len: nat)
+  requires NoDuplicates(xs)
+  requires forall x :: x in Elements(xs) ==> (AbLt(n, x) || n == x)
+  requires len == Length(xs)
+  ensures var s := SMN''(xs, n, len);
+    (AbLt(n, s) || n == s) &&
+    (AbLt(s, AbAdd(n, int2adt(len))) || s == AbAdd(n, int2adt(len))) &&
+    s !in Elements(xs) &&
+    forall x :: (AbLt(n, x) || n == x) && AbLt(x, s) ==> x in Elements(xs)
+  decreases len
+{
+  Props ();
+  if xs == Nil {
+  } else {
+    var half := len / 2 + 1;
+    var (L, R) := Split(xs, AbAdd(n, int2adt(half)));
+    Split_Correct(xs, AbAdd(n, int2adt(half)));
+    var llen := Length(L);
+    Elements_Property(L);  // use the NoDuplicates property
+    var bound := IntRange(n, half);
+    Cardinality(Elements(L), bound);
+    if llen < half {
+      SMN''_Correct(L, n, llen);
+    } else {
+      var s := SMN''(R, AbAdd(n, int2adt(llen)), len - llen);
+      SMN''_Correct(R, AbAdd(n, int2adt(llen)), len - llen);
+      forall x | (AbLt(n, x) || n == x) && AbLt(x, s)
+        ensures x in Elements(xs)
+      {
+        if AbLt(x, AbAdd(n, int2adt(llen))) {
+          SetEquality(Elements(L), bound);
+        }
+      }
+    }
+  }
+}
